feat(lean_chacha20): use new attributes

hax-lib/proof-libs/lean/Hax/rust_primitives/sequence.lean
@@ -1,20 +1,30 @@
 import Hax.rust_primitives.RustM
 import Hax.rust_primitives.num
 
-abbrev rust_primitives.sequence.Seq α := Array α
+structure rust_primitives.sequence.Seq α where
+  val : Array α
+  size_lt_usizeSize : val.size < USize64.size
+
+attribute [grind .] rust_primitives.sequence.Seq.size_lt_usizeSize
+attribute [local grind! .] USize64.toNat_lt_size
+
+@[grind =, simp]
+theorem rust_primitives.sequence.Seq.toNat_ofNat_size {α} (m : rust_primitives.sequence.Seq α) :
+    (USize64.ofNat m.val.size).toNat = m.val.size :=
+  USize64.toNat_ofNat_of_lt' m.size_lt_usizeSize
 
 def rust_primitives.sequence.seq_len (α : Type) (s : rust_primitives.sequence.Seq α) :
-  RustM usize := pure (USize64.ofNat (Array.size s))
+  RustM usize := pure (USize64.ofNat s.val.size)
 
 def rust_primitives.sequence.seq_first (α : Type) (s : rust_primitives.sequence.Seq α) : RustM α :=
-  if h : s.size == 0 then
+  if h : s.val.size == 0 then
     .fail .arrayOutOfBounds
   else
-    pure (s[0]'(by grind))
+    pure (s.val[0]'(by grind))
 
 def rust_primitives.sequence.seq_slice
   (α : Type) (seq : rust_primitives.sequence.Seq α) (s e : usize) : RustM (rust_primitives.sequence.Seq α) :=
-  if s ≤ e && e ≤ .ofNat seq.size then
-    pure seq[s.toNat:e.toNat].toArray
+  if s ≤ e && e ≤ .ofNat seq.val.size then
+    pure ⟨seq.val[s.toNat:e.toNat].toArray, by grind⟩
   else
     .fail .undef
