hax-lib/proof-libs/lean/Hax/core_models/epilogue/alloc.lean
@@ -11,21 +11,32 @@ Rust vectors are represented as Lean Arrays (variable size)
 -/
 section RustVectors
 
+open rust_primitives.sequence
+
 def alloc.alloc.Global : Type := Unit
 
-abbrev alloc.vec.Vec (α: Type) (_Allocator:Type) : Type := Array α
+abbrev alloc.vec.Vec (α: Type) (_Allocator:Type) : Type := Seq α
 
+@[spec]
 def alloc.vec.Impl.new (α: Type) (_:Tuple0) : RustM (alloc.vec.Vec α alloc.alloc.Global) :=
-  pure ((List.nil).toArray)
+  pure ⟨(List.nil).toArray, by grind⟩
 
+@[spec]
 def alloc.vec.Impl_1.len (α: Type) (_Allocator: Type) (x: alloc.vec.Vec α alloc.alloc.Global) : RustM usize :=
-  pure (.ofNat x.size)
+  pure (.ofNat x.val.size)
 
-def alloc.vec.Impl_2.extend_from_slice α (_Allocator: Type) (x: alloc.vec.Vec α alloc.alloc.Global) (y: Array α)
-  : RustM (alloc.vec.Vec α alloc.alloc.Global):=
-  pure (x.append y)
+@[spec]
+def alloc.vec.Impl_2.extend_from_slice α (_Allocator: Type)
+    (x: alloc.vec.Vec α alloc.alloc.Global) (y: Seq α) :
+    RustM (alloc.vec.Vec α alloc.alloc.Global) :=
+  if h : x.val.size + y.val.size < USize64.size then
+    pure ⟨x.val.append y.val, by simp [h]⟩
+  else
+    .fail .maximumSizeExceeded
 
-def alloc.slice.Impl.to_vec α (a:  Array α) : RustM (alloc.vec.Vec α alloc.alloc.Global) :=
+@[spec]
+def alloc.slice.Impl.to_vec α (a: rust_primitives.sequence.Seq α) :
+    RustM (alloc.vec.Vec α alloc.alloc.Global) :=
   pure a
 
 end RustVectors
