hax-lib/proof-libs/lean/Hax/rust_primitives/slice.lean
@@ -3,13 +3,17 @@ import Hax.rust_primitives.hax
 import Hax.rust_primitives.sequence
 
 
-abbrev RustSlice := Array
-abbrev RustVector := Array
+
+abbrev RustVector := rust_primitives.sequence.Seq
+abbrev RustSlice := rust_primitives.sequence.Seq
+
+attribute [local grind! .] rust_primitives.sequence.Seq.size_lt_usizeSize
+attribute [local grind! .] USize64.toNat_lt_size
 
 @[spec]
 def rust_primitives.slice.array_as_slice (α : Type) (n : usize) :
     RustArray α n → RustM (RustSlice α) :=
-  fun x => pure (Vector.toArray x)
+  fun x => pure ⟨Vector.toArray x, by grind⟩
 
 @[spec]
 def rust_primitives.slice.array_map (α : Type) (β : Type) (n : usize) (_ : Type)
@@ -23,7 +27,7 @@ def rust_primitives.slice.array_from_fn (α : Type) (n : usize) (_ : Type)
 
 @[spec]
 def rust_primitives.slice.slice_length (α : Type) (s : RustSlice α) : RustM usize :=
-  pure (USize64.ofNat s.size)
+  pure (USize64.ofNat s.val.size)
 
 @[spec]
 def rust_primitives.sequence.seq_from_slice (α : Type) (s : RustSlice α) :
@@ -33,14 +37,14 @@ def rust_primitives.sequence.seq_from_slice (α : Type) (s : RustSlice α) :
 @[spec]
 def rust_primitives.slice.slice_split_at (α : Type) (s : RustSlice α) (mid : usize) :
     RustM (rust_primitives.hax.Tuple2 (RustSlice α) (RustSlice α)) :=
-  if mid <= .ofNat s.size then
-    pure ⟨s.take mid.toNat, s.drop mid.toNat⟩
+  if mid <= .ofNat s.val.size then
+    pure ⟨⟨s.val.take mid.toNat, by grind⟩, ⟨s.val.drop mid.toNat, by grind⟩⟩
   else
     .fail .arrayOutOfBounds
 
 def rust_primitives.slice.slice_slice
   (α : Type) (seq : RustSlice α) (s e : usize) : RustM (RustSlice α) :=
-  if s ≤ e && e ≤ .ofNat seq.size then
-    pure seq[s.toNat:e.toNat].toArray
+  if s ≤ e && e ≤ .ofNat seq.val.size then
+    pure ⟨seq.val[s.toNat:e.toNat].toArray, by grind⟩
   else
     .fail .undef
